more array examples

ArrayExamples.dfy
@@ -1,11 +1,10 @@
-// RUN: /compile:0
+// RUN: /compile:0 /rlimit:1000000
 
 method ArrayInit<A>(f: int -> A, a: array<A>)
     requires a != null
     requires forall x :: 0 <= x < a.Length ==> f.requires(x)
     requires forall x :: 0 <= x < a.Length ==> a !in f.reads(x)
     modifies a
-    ensures forall x :: 0 <= x < a.Length ==> f.requires(x)
     ensures forall x :: 0 <= x < a.Length ==> a[x] == f(x)
 {
     var i := 0;
@@ -229,6 +228,7 @@ method Insert<A>(cmp: (A, A) -> bool, a: array<A>, i: int)
     modifies a
     ensures forall x :: 0 <= x < a.Length ==> a[x] in old(a[..])
     ensures forall x, y :: 0 <= x < y <= i ==> cmp(a[x], a[y])
+    ensures multiset(a[..]) == old(multiset(a[..]))
 {
     var j := i - 1;
     while j >= 0 && !cmp(a[j], a[j + 1])
@@ -238,6 +238,7 @@ method Insert<A>(cmp: (A, A) -> bool, a: array<A>, i: int)
         invariant forall x, y :: 0 <= x < y <= j ==> cmp(a[x], a[y])
         invariant forall x, y :: j < x < y <= i ==> cmp(a[x], a[y])
         invariant forall x, y :: 0 <= x < j + 1 < y <= i ==> cmp(a[x], a[y])
+        invariant multiset(a[..]) == old(multiset(a[..]))
     {
         a[j], a[j+1] := a[j+1], a[j];
         j := j - 1;
@@ -245,7 +246,7 @@ method Insert<A>(cmp: (A, A) -> bool, a: array<A>, i: int)
 }
 
 method GenericSort<A>(cmp: (A, A) -> bool, a: array<A>)
-    requires a != null && a.Length > 0
+    requires a != null
     requires forall x, y :: x in a[..] && y in a[..] ==> a !in cmp.reads(x, y)
     requires forall x, y :: x in a[..] && y in a[..] ==> cmp.requires(x, y)
     requires forall x, y :: x in a[..] && y in a[..] ==> cmp(x, y) || cmp(y, x)
@@ -253,6 +254,7 @@ method GenericSort<A>(cmp: (A, A) -> bool, a: array<A>)
     modifies a
     ensures forall x :: 0 <= x < a.Length ==> a[x] in old(a[..])
     ensures forall x, y :: 0 <= x < y < a.Length ==> cmp(a[x], a[y])
+    ensures multiset(a[..]) == old(multiset(a[..]))
 {
     var i := 0;
     while i < a.Length
@@ -260,8 +262,139 @@ method GenericSort<A>(cmp: (A, A) -> bool, a: array<A>)
         invariant 0 <= i <= a.Length
         invariant forall x :: 0 <= x < a.Length ==> a[x] in old(a[..])
         invariant forall x, y :: 0 <= x < y < i ==> cmp(a[x], a[y])
+        invariant multiset(a[..]) == old(multiset(a[..]))
     {
         Insert(cmp, a, i);
         i := i + 1;
     }
+}
+
+function method Range(start: int, length: nat): seq<int>
+    decreases length
+{
+    if length == 0 then
+        []
+    else 
+        [start] + Range(start + 1, length -1)
+}
+
+lemma lemma_RangeLength(start: int, length: nat)
+    decreases length
+    ensures |Range(start, length)| == length
+{}
+
+lemma lemma_RangeIndex(start: int, length: nat)
+    decreases length
+    ensures (lemma_RangeLength(start, length); forall i :: 0 <= i < length ==> Range(start, length)[i] == start + i)
+{}
+
+lemma lemma_SeqExt<A>(l1: seq<A>, l2: seq<A>)
+    requires |l1| == |l2|
+    requires forall i :: 0 <= i < |l1| ==> l1[i] == l2[i]
+    ensures l1 == l2
+{}
+
+function Reverse<A>(l: seq<A>): seq<A>
+{
+    if l == [] then
+        []
+    else 
+        Reverse(l[1..]) + [l[0]]
+}
+
+lemma lemma_ReverseLength<A>(l: seq<A>)
+    ensures |Reverse(l)| == |l|
+{}
+
+lemma lemma_ReversePlus<A>(l1: seq<A>, l2: seq<A>)
+    ensures Reverse(l1 + l2) == Reverse(l2) + Reverse(l1)
+{
+    if l1 != [] {
+        assert (l1 + l2)[1..] == l1[1..] + l2;
+    }
+}
+
+lemma lemma_ReverseIndex<A>(l: seq<A>, i: int)
+    requires 0 <= i < |l|
+    ensures (lemma_ReverseLength(l); Reverse(l)[i] == l[|l| - i - 1])
+{
+    lemma_ReverseLength(l);
+}
+
+lemma lemma_ReverseReverse<A>(l: seq<A>)
+    ensures Reverse(Reverse(l)) == l
+{
+    lemma_ReverseLength(l);
+    lemma_ReverseLength(Reverse(l));
+    
+    forall i | 0 <= i < |l| ensures Reverse(Reverse(l))[i] == l[i]
+    {
+        calc {
+            Reverse(Reverse(l))[i]; 
+                {lemma_ReverseIndex(Reverse(l), i);}
+            Reverse(l)[|l| - i - 1];
+                {lemma_ReverseIndex(l, |l| - i - 1);}
+            l[i];
+        }
+    }
+
+    lemma_SeqExt(Reverse(Reverse(l)), l);
+}
+
+lemma lemma_MultisetSeqRest<A>(l: seq<A>)
+    requires l != []
+    ensures multiset(l[1..]) == multiset(l) - multiset{l[0]}
+{
+    calc {
+        multiset(l[1..]);
+        multiset([l[0]] + l[1..]) - multiset{l[0]}; { assert l == [l[0]] + l[1..]; }
+        multiset(l) - multiset{l[0]};
+    }
+}
+
+lemma lemma_SortedUnique<A>(cmp: (A, A) -> bool, l1: seq<A>, l2: seq<A>)
+    requires |l1| == |l2|
+    requires multiset(l1) == multiset(l2)
+
+    requires forall x, y :: x in l1 + l2 && y in l1 + l2 ==> cmp.requires(x, y)
+    requires forall x :: x in l1 + l2 ==> cmp.requires(x, x) && cmp(x, x)
+    requires forall x, y :: x in l1 + l2 && y in l1 + l2 ==> cmp(x, y) && cmp(y, x) ==> x == y
+
+    requires forall x, y :: 0 <= x < y < |l1| ==> cmp(l1[x], l1[y])
+    requires forall x, y :: 0 <= x < y < |l2| ==> cmp(l2[x], l2[y])
+    
+    ensures l1 == l2
+{
+    if l1 != [] {
+        assert forall x :: x in l1 ==> cmp(l1[0], x);
+        assert forall x :: x in l2 ==> cmp(l2[0], x);
+        assert l1[0] in multiset(l2) && l2[0] in multiset(l1);
+        assert cmp(l1[0], l2[0]) && cmp(l2[0], l1[0]);
+        assert l1[0] == l2[0];
+        calc {
+            multiset(l1[1..]); 
+                { lemma_MultisetSeqRest(l1); }
+            multiset(l1) - multiset{l1[0]};
+            multiset(l2) - multiset{l2[0]}; 
+                { lemma_MultisetSeqRest(l2); }
+            multiset(l2[1..]);
+        }
+        lemma_SortedUnique(cmp, l1[1..], l2[1..]);
+    }
+}
+
+method Main(n: nat)
+{
+    var a := new int[n];
+    ArrayInit((i: int) => i, a);
+
+    lemma_RangeLength(0, n);
+    lemma_RangeIndex(0, n);
+    lemma_SeqExt(a[..], Range(0, n));
+    assert a[..] == Range(0, n);
+    
+    var le := (x, y) => x <= y;
+    GenericSort(le, a);
+    lemma_SortedUnique(le, a[..], Range(0, n));
+    assert a[..] == Range(0, n); 
 }
